theories/simplang/examples/sum.v
@@ -1,7 +1,7 @@
-From simuliris.simplang Require Import lang notation tactics class_instances proofmode.
 From iris Require Import bi.bi.
 From iris.proofmode Require Import tactics.
 From simuliris.simulation Require Import slsls lifting.
+From simuliris.simplang Require Import lang notation tactics class_instances proofmode.
 From iris.prelude Require Import options.
 
 Import bi.
