theories/simplang/gen_refl.v
@@ -1,6 +1,6 @@
-From simuliris.simulation Require Import slsls lifting.
+From simuliris.simulation Require Import slsls lifting gen_log_rel.
 From simuliris.simplang Require Import proofmode tactics.
-From simuliris.simplang Require Import primitive_laws gen_val_rel gen_log_rel wf.
+From simuliris.simplang Require Import primitive_laws gen_val_rel wf.
 From iris.prelude Require Import options.
 
 (** * Lemmas for proving [log_rel]
@@ -10,16 +10,18 @@ From iris.prelude Require Import options.
 
 Section log_rel.
   Context `{!sheapGS Σ} `{!sheapInv Σ}.
+  (* TODO: can we avoid this boilerplate? It is repeated in all files that
+     are generic over the logical relation details. *)
   Context (loc_rel : loc → loc → iProp Σ) {Hpers : ∀ l_t l_s, Persistent (loc_rel l_t l_s)}.
   Context (thread_own : thread_id → iProp Σ).
-  Let val_rel := (gen_val_rel loc_rel).
-  Let log_rel := (gen_log_rel loc_rel thread_own).
+  Local Notation val_rel := (gen_val_rel loc_rel).
+  Local Notation log_rel := (gen_log_rel val_rel thread_own).
 
   Lemma val_wf_sound v : val_wf v → ⊢ val_rel v v.
-  Proof using Hpers.
+  Proof.
     intros Hv.
     iInduction v as [[] | | | ] "IH"; try by (simpl; try iApply "IH").
-    simpl. destruct Hv as [H1 H2]. iSplit; [by iApply "IH" | by iApply "IH1"].
+    simpl. destruct Hv as [H1 H2]. iSplitL; [by iApply "IH" | by iApply "IH1"].
   Qed.
 
   Local Lemma call_not_val v1 v2 : language.to_val (Call v1 v2) = None.
@@ -50,7 +52,8 @@ Section log_rel.
     iApply (sim_wand with Hp).
 
   Lemma log_rel_var x : ⊢ log_rel (Var x) (Var x).
-  Proof using Hpers.
+  Proof.
+    clear Hpers. rewrite /gen_log_rel.
     iIntros (? xs) "!# Hs Ht"; simpl.
     iDestruct (subst_map_rel_lookup _ x with "Hs") as (v_t v_s Hv) "Hrel"; first set_solver.
     rewrite !lookup_fmap Hv /=. sim_val. by iFrame.
@@ -59,14 +62,15 @@ Section log_rel.
   Lemma log_rel_let x e1_t e1_s e2_t e2_s :
     log_rel e1_t e1_s -∗ log_rel e2_t e2_s -∗ log_rel (Let x e1_t e2_t) (Let x e1_s e2_s).
   Proof using Hpers.
+    rewrite /gen_log_rel.
     iIntros "#IH1 #IH2" (? xs) "!# #Hs Ht"; simpl.
-    smart_sim_bind (subst_map _ _) (subst_map _ _) "(IH1 [] Ht)".
+    smart_sim_bind (subst_map _ _) (subst_map _ _) "(IH1 [Hs] Ht)".
     { iApply (subst_map_rel_weaken with "[$]"). set_solver. }
     iIntros (v_t v_s) "[Ht #Hv]". sim_pures. rewrite !subst'_subst_map.
     rewrite -(binder_insert_fmap fst (v_t, v_s)).
     rewrite -(binder_insert_fmap snd (v_t, v_s)).
     iApply ("IH2" with "[] Ht").
-    iApply (subst_map_rel_insert with "[] Hv").
+    iApply (subst_map_rel_insert with "[] [Hv]"); last done.
     iApply (subst_map_rel_weaken with "[$]").
     destruct x as [|x]; first set_solver.
     apply elem_of_subseteq=>x'.
@@ -77,6 +81,7 @@ Section log_rel.
     (∀ π v_t v_s, ext_rel π v_t v_s ⊣⊢ thread_own π ∗ val_rel v_t v_s) →
     log_rel e1_t e1_s -∗ log_rel e2_t e2_s -∗ log_rel (Call e1_t e2_t) (Call e1_s e2_s).
   Proof using Hpers.
+    rewrite /gen_log_rel.
     iIntros (Hext) "#IH1 #IH2". iIntros (? xs) "!# #Hs Ht"; simpl.
     smart_sim_bind (subst_map _ _) (subst_map _ _) "(IH2 [] Ht)".
     { iApply (subst_map_rel_weaken with "[$]"). set_solver. }
@@ -90,11 +95,12 @@ Section log_rel.
 
   Lemma log_rel_unop e_t e_s o :
     log_rel e_t e_s -∗ log_rel (UnOp o e_t) (UnOp o e_s).
-  Proof using Hpers.
-    iIntros "#IH" (? xs) "!# #Hs Ht"; simpl.
-    smart_sim_bind (subst_map _ e_t) (subst_map _ e_s) "(IH [] Ht)".
+  Proof.
+    clear Hpers. rewrite /gen_log_rel.
+    iIntros "#IH" (? xs) "!# Hs Ht"; simpl.
+    smart_sim_bind (subst_map _ e_t) (subst_map _ e_s) "(IH [Hs] Ht)".
     { iApply (subst_map_rel_weaken with "[$]"). set_solver. }
-    iIntros (v_t v_s) "[Ht #Hv]".
+    iIntros (v_t v_s) "[Ht Hv]".
     destruct o; sim_pures; discr_source; val_discr_source "Hv"; sim_pures; sim_val; by iFrame.
   Qed.
 
@@ -104,6 +110,7 @@ Section log_rel.
     loc_rel_offset_law loc_rel →
     log_rel e1_t e1_s -∗ log_rel e2_t e2_s -∗ log_rel (BinOp o e1_t e2_t) (BinOp o e1_s e2_s).
   Proof using Hpers.
+    rewrite /gen_log_rel.
     iIntros (Hfunc Hinj Hshift). iIntros "#IH1 #IH2" (? xs) "!# #Hs Ht"; simpl.
     smart_sim_bind (subst_map _ e2_t) (subst_map _ e2_s) "(IH2 [] Ht)".
     { iApply (subst_map_rel_weaken with "[$]"). set_solver. }
@@ -143,6 +150,7 @@ Section log_rel.
     log_rel e3_t e3_s -∗
     log_rel (If e1_t e2_t e3_t) (If e1_s e2_s e3_s).
   Proof using Hpers.
+    rewrite /gen_log_rel.
     iIntros "#IH1 #IH2 #IH3" (? xs) "!# #Hs Ht"; simpl.
     smart_sim_bind (subst_map _ e1_t) (subst_map _ e1_s) "(IH1 [] Ht)".
     { iApply (subst_map_rel_weaken with "[$]"). set_solver. }
@@ -158,6 +166,7 @@ Section log_rel.
     log_rel e2_t e2_s -∗
     log_rel (While e1_t e2_t) (While e1_s e2_s).
   Proof using Hpers.
+    rewrite /gen_log_rel.
     iIntros "#IH1 #IH2" (? xs) "!# #Hs Ht"; simpl.
     iApply (sim_while_while _ _ _ _ _ (thread_own _)%I with "[$]").
     iModIntro; iIntros "Ht".
@@ -178,6 +187,7 @@ Section log_rel.
     log_rel e2_t e2_s -∗
     log_rel (Pair e1_t e2_t) (Pair e1_s e2_s).
   Proof using Hpers.
+    rewrite /gen_log_rel.
     iIntros "#IH1 #IH2" (? xs) "!# #Hs Ht"; simpl.
     smart_sim_bind (subst_map _ e2_t) (subst_map _ e2_s) "(IH2 [] Ht)".
     { iApply (subst_map_rel_weaken with "[$]"). set_solver. }
@@ -190,9 +200,10 @@ Section log_rel.
 
   Lemma log_rel_fst e_t e_s :
     log_rel e_t e_s -∗ log_rel (Fst e_t) (Fst e_s).
-  Proof using Hpers.
-    iIntros "#IH" (? xs) "!# #Hs Ht"; simpl.
-    smart_sim_bind (subst_map _ e_t) (subst_map _ e_s) "(IH [] Ht)".
+  Proof.
+    clear Hpers. rewrite /gen_log_rel.
+    iIntros "#IH" (? xs) "!# Hs Ht"; simpl.
+    smart_sim_bind (subst_map _ e_t) (subst_map _ e_s) "(IH [Hs] Ht)".
     { iApply (subst_map_rel_weaken with "[$]"). set_solver. }
     iIntros (v_t v_s) "[Ht Hv]".
     discr_source.
@@ -200,9 +211,10 @@ Section log_rel.
   Qed.
   Lemma log_rel_snd e_t e_s :
     log_rel e_t e_s -∗ log_rel (Snd e_t) (Snd e_s).
-  Proof using Hpers.
-    iIntros "#IH" (? xs) "!# #Hs Ht"; simpl.
-    smart_sim_bind (subst_map _ e_t) (subst_map _ e_s) "(IH [] Ht)".
+  Proof.
+    clear Hpers. rewrite /gen_log_rel.
+    iIntros "#IH" (? xs) "!# Hs Ht"; simpl.
+    smart_sim_bind (subst_map _ e_t) (subst_map _ e_s) "(IH [Hs] Ht)".
     { iApply (subst_map_rel_weaken with "[$]"). set_solver. }
     iIntros (v_t v_s) "[Ht Hv]".
     discr_source.
@@ -212,6 +224,7 @@ Section log_rel.
   Lemma log_rel_injl e_t e_s :
     log_rel e_t e_s -∗ log_rel (InjL e_t) (InjL e_s).
   Proof using Hpers.
+    rewrite /gen_log_rel.
     iIntros "#IH" (? xs) "!# #Hs Ht"; simpl.
     smart_sim_bind (subst_map _ e_t) (subst_map _ e_s) "(IH [] Ht)".
     { iApply (subst_map_rel_weaken with "[$]"). set_solver. }
@@ -220,6 +233,7 @@ Section log_rel.
   Lemma log_rel_injr e_t e_s :
     log_rel e_t e_s -∗ log_rel (InjR e_t) (InjR e_s).
   Proof using Hpers.
+    rewrite /gen_log_rel.
     iIntros "#IH" (? xs) "!# #Hs Ht"; simpl.
     smart_sim_bind (subst_map _ e_t) (subst_map _ e_s) "(IH [] Ht)".
     { iApply (subst_map_rel_weaken with "[$]"). set_solver. }
@@ -232,6 +246,7 @@ Section log_rel.
     log_rel e2_t e2_s -∗
     log_rel (Match e_t x1 e1_t x2 e2_t) (Match e_s x1 e1_s x2 e2_s).
   Proof using Hpers.
+    rewrite /gen_log_rel.
     iIntros "#IH #IH1 #IH2" (? xs) "!# #Hs Ht"; simpl.
     smart_sim_bind (subst_map _ e_t) (subst_map _ e_s)  "(IH [] Ht)".
     { iApply (subst_map_rel_weaken with "[$]"). set_solver. }
@@ -245,7 +260,7 @@ Section log_rel.
       rewrite -(binder_insert_fmap fst (v_t', v_s')).
       rewrite -(binder_insert_fmap snd (v_t', v_s')).
       iApply ("IH1" with "[] Ht").
-      iApply (subst_map_rel_insert with "[] [//]").
+      iApply (subst_map_rel_insert with "[] []"); last done.
       iApply (subst_map_rel_weaken with "[$]").
       destruct x1 as [|x1]; first set_solver.
       apply elem_of_subseteq=>x'.
@@ -258,7 +273,7 @@ Section log_rel.
       rewrite -(binder_insert_fmap fst (v_t', v_s')).
       rewrite -(binder_insert_fmap snd (v_t', v_s')).
       iApply ("IH2" with "[] Ht").
-      iApply (subst_map_rel_insert with "[] [//]").
+      iApply (subst_map_rel_insert with "[] []"); last done.
       iApply (subst_map_rel_weaken with "[$]").
       destruct x2 as [|x2]; first set_solver.
       apply elem_of_subseteq=>x'.
@@ -273,6 +288,7 @@ Section log_rel.
      Fork e_t ⪯{π} Fork e_s [{ Ψ }]) →
     log_rel e_t e_s -∗ log_rel (Fork e_t) (Fork e_s).
   Proof using Hpers.
+    rewrite /gen_log_rel.
     iIntros (Hfork). iIntros "#IH" (? xs) "!# #Hs Ht"; simpl.
     iApply (Hfork with "Ht"); first by iIntros "?"; sim_pures; sim_val; iFrame.
     iIntros (?) "Ht". iApply (sim_wand with "(IH [] Ht)"); eauto.
@@ -285,6 +301,7 @@ Section log_rel.
      AllocN #n v_t ⪯{π} AllocN #n v_s [{ Ψ }]) →
     log_rel e1_t e1_s -∗ log_rel e2_t e2_s -∗ log_rel (AllocN e1_t e2_t) (AllocN e1_s e2_s).
   Proof using Hpers.
+    rewrite /gen_log_rel.
     iIntros (Halloc). iIntros "#IH1 #IH2" (? xs) "!# #Hs Ht"; simpl.
     smart_sim_bind (subst_map _ e2_t) (subst_map _ e2_s) "(IH2 [] Ht)".
     { iApply (subst_map_rel_weaken with "[$]"). set_solver. }
@@ -304,6 +321,7 @@ Section log_rel.
      FreeN #n #l_t ⪯{π} FreeN #n #l_s [{ Ψ }]) →
     log_rel e1_t e1_s -∗ log_rel e2_t e2_s -∗ log_rel (FreeN e1_t e2_t) (FreeN e1_s e2_s).
   Proof using Hpers.
+    rewrite /gen_log_rel.
     iIntros (Hfree). iIntros "#IH1 #IH2" (? xs) "!# #Hs Ht"; simpl.
     smart_sim_bind (subst_map _ _) (subst_map _ _) "(IH2 [] Ht)".
     { iApply (subst_map_rel_weaken with "[$]"). set_solver. }
@@ -324,6 +342,7 @@ Section log_rel.
      Load o #l_t ⪯{π} Load o #l_s [{ Ψ }]) →
     log_rel e_t e_s -∗ log_rel (Load o e_t) (Load o e_s).
   Proof using Hpers.
+    rewrite /gen_log_rel.
     iIntros (Hload). iIntros "#IH" (? xs) "!# #Hs Ht"; simpl.
     smart_sim_bind (subst_map _ _) (subst_map _ _) "(IH [] Ht)".
     { iApply (subst_map_rel_weaken with "[$]"). set_solver. }
@@ -340,6 +359,7 @@ Section log_rel.
      Store o #l_t v_t ⪯{π} Store o #l_s v_s [{ Ψ }]) →
     log_rel e1_t e1_s -∗ log_rel e2_t e2_s -∗ log_rel (Store o e1_t e2_t) (Store o e1_s e2_s).
   Proof using Hpers.
+    rewrite /gen_log_rel.
     iIntros (Hstore). iIntros "#IH1 #IH2" (? xs) "!# #Hs Ht"; simpl.
     smart_sim_bind (subst_map _ _) (subst_map _ _) "(IH2 [] Ht)".
     { iApply (subst_map_rel_weaken with "[$]"). set_solver. }
@@ -355,6 +375,7 @@ Section log_rel.
   Lemma log_rel_val v_t v_s :
     val_rel v_t v_s -∗ log_rel (Val v_t) (Val v_s).
   Proof using Hpers.
-    iIntros "#Hv" (? xs) "!# #Hs Ht"; simpl. sim_val; by iFrame.
+    rewrite /gen_log_rel.
+    iIntros "#Hv" (? xs) "!# Hs Ht"; simpl. sim_val; by iFrame.
   Qed.
 End log_rel.
