theories/simplang/na_inv/examples/data_races.v
@@ -1,7 +1,8 @@
-From simuliris.simplang Require Import lang notation tactics class_instances proofmode gen_log_rel wf.
 From iris Require Import bi.bi.
 From iris.proofmode Require Import tactics.
 From simuliris.simulation Require Import slsls lifting.
+From simuliris.simplang Require Import lang notation tactics class_instances
+  proofmode log_rel_structural wf.
 From simuliris.simplang.na_inv Require Export inv.
 From simuliris.simplang.na_inv Require Import readonly_refl adequacy.
 From iris.prelude Require Import options.
