theories/simplang/na_inv/inv.v
@@ -2,10 +2,10 @@ From iris.proofmode Require Import tactics.
 From iris.bi.lib Require Import fractional .
 From iris.base_logic.lib Require Import ghost_map.
 From simuliris.base_logic Require Export gen_sim_heap gen_sim_prog.
-From simuliris.simulation Require Import slsls lifting.
+From simuliris.simulation Require Import slsls lifting gen_log_rel.
 From iris.algebra.lib Require Import gset_bij.
 From iris.base_logic.lib Require Import gset_bij.
-From simuliris.simplang Require Export class_instances primitive_laws heapbij gen_val_rel gen_log_rel globalbij.
+From simuliris.simplang Require Export class_instances primitive_laws heapbij gen_val_rel globalbij.
 From simuliris.simplang.na_inv Require Export na_locs.
 
 From iris.prelude Require Import options.
@@ -66,7 +66,7 @@ Section laws.
 End laws.
 
 Notation val_rel := (gen_val_rel heapbij.loc_rel).
-Notation log_rel := (gen_log_rel heapbij.loc_rel (λ π, na_locs π ∅)).
+Notation log_rel := (gen_log_rel val_rel (λ π, na_locs π ∅)).
 
 Section fix_heap.
   Context `{naGS Σ}.
