theories/simulation/gen_log_rel.v
@@ -1,0 +1,211 @@
+
+From stdpp Require Import binders.
+From iris.bi Require Import bi.
+From iris.proofmode Require Import tactics.
+From simuliris.simulation Require Import relations language.
+From simuliris.simulation Require Export simulation slsls.
+From iris.prelude Require Import options.
+Import bi.
+
+(** * Logical relation
+
+    General definition of [log_rel] which lifts the simulation relation (the
+    "expression relation") to open terms.on open terms. *)
+
+Section fix_lang.
+  Context {PROP : bi} `{!BiBUpd PROP, !BiAffine PROP, !BiPureForall PROP}.
+  Context {Λ : language}.
+  Context `{!simulirisGS PROP Λ}.
+
+  Set Default Proof Using "Type*".
+
+  Implicit Types
+    (e_s e_t e: expr Λ)
+    (P_s P_t P: prog Λ)
+    (σ_s σ_t σ : state Λ).
+
+  (** Whole-program relation *)
+  Definition prog_rel P_t P_s : PROP :=
+    (□ ∀ f x_s e_s, ⌜P_s !! f = Some (x_s, e_s)⌝ →
+       ∃ x_t e_t, ⌜P_t !! f = Some (x_t, e_t)⌝ ∗
+         ∀ v_t v_s π, ext_rel π v_t v_s -∗
+           (subst_map {[x_t:=v_t]} e_t) ⪯{π} (subst_map {[x_s:=v_s]} e_s) {{ ext_rel π }})%I.
+  Typeclasses Opaque prog_rel.
+
+  Global Instance prog_rel_persistent P_t P_s : Persistent (prog_rel P_t P_s).
+  Proof. rewrite /prog_rel; apply _. Qed.
+
+  
+  (** Relation on "contexts", lifted from a value relation:
+      Well-formed substitutions closing source and target, with [X] denoting the
+      free variables. *)
+  Context (val_rel : val Λ → val Λ → PROP).
+
+  Definition subst_map_rel (X : gset string) (map : gmap string (val Λ * val Λ)) : PROP :=
+    [∗ set] x ∈ X,
+      match map !! x with
+      | Some (v_t, v_s) => val_rel v_t v_s
+      | None => False
+      end.
+
+  Global Instance subst_map_rel_pers X map `{!∀ vt vs, Persistent (val_rel vt vs)} :
+    Persistent (subst_map_rel X map).
+  Proof.
+    rewrite /subst_map_rel. apply big_sepS_persistent=>x.
+    destruct (map !! x) as [[v_t v_s]|]; apply _.
+  Qed.
+
+  Lemma subst_map_rel_lookup {X map} x :
+    x ∈ X →
+    subst_map_rel X map -∗
+    ∃ v_t v_s, ⌜map !! x = Some (v_t, v_s)⌝ ∗ val_rel v_t v_s.
+  Proof.
+    iIntros (Hx) "Hrel".
+    iDestruct (big_sepS_elem_of _ _ x with "Hrel") as "Hrel"; first done.
+    destruct (map !! x) as [[v_t v_s]|]; last done. eauto.
+  Qed.
+
+  Lemma subst_map_rel_weaken X1 X2 map :
+    X2 ⊆ X1 →
+    subst_map_rel X1 map -∗ subst_map_rel X2 map.
+  Proof. iIntros (HX). iApply big_sepS_subseteq. done. Qed.
+
+  Lemma subst_map_rel_singleton X x v_t v_s :
+    X ⊆ {[x]} →
+    val_rel v_t v_s -∗
+    subst_map_rel X {[x:=(v_t, v_s)]}.
+  Proof.
+    iIntros (?) "Hrel".
+    iApply (subst_map_rel_weaken {[x]}); first done.
+    rewrite /subst_map_rel big_sepS_singleton lookup_singleton. done.
+  Qed.
+
+  (* TODO: use [binder_delete], once we can [delete] on [gset]. *)
+  Definition binder_delete_gset (b : binder) (X : gset string) :=
+    match b with BAnon => X | BNamed x => X ∖ {[x]} end.
+
+  (* TODO upstream to Iris *)
+  Lemma big_sepS_delete_2 `{Countable A} (Φ : A → PROP) (X : gset A) x :
+    Φ x ∗ ([∗ set] y ∈ X ∖ {[ x ]}, Φ y) ⊢ [∗ set] y ∈ X, Φ y.
+  Proof.
+    destruct (decide (x ∈ X)).
+    - rewrite -big_sepS_delete //.
+    - replace (X ∖ {[x]}) with X by set_solver.
+      rewrite bi.sep_elim_r. done.
+  Qed.
+
+  Lemma subst_map_rel_insert X x v_t v_s map :
+    subst_map_rel (binder_delete_gset x X) map -∗
+    val_rel v_t v_s -∗
+    subst_map_rel X (binder_insert x (v_t, v_s) map).
+  Proof.
+    iIntros "Hmap Hval". destruct x as [|x]; first done. simpl.
+    rewrite /subst_map_rel. rewrite -(big_sepS_delete_2 _ X x).
+    iSplitL "Hval".
+    - rewrite lookup_insert. done.
+    - iApply (big_sepS_impl with "Hmap").
+      iIntros "!# %x' %Hx'".
+      destruct (decide (x = x')) as [<-|Hne]; first by set_solver.
+      rewrite lookup_insert_ne //. auto.
+  Qed.
+
+  Lemma subst_map_rel_empty map :
+    ⊢ subst_map_rel ∅ map.
+  Proof. iApply big_sepS_empty. done. Qed.
+
+  (** The core "logical relation" of our system:
+      The simulation relation ("expression relation") must hold after applying
+      an arbitrary well-formed closing substitution [map].
+
+      We might define multiple logical relations for the same Simuliris
+      instance, so this is parameterized separately. The "main" logical relation
+      will usually choose these such that [ext_rel = val_rel ∗ thread_own], but
+      further auxiliary logical relations might make different choices. *)
+  (* TODO: make this not persistent? *)
+  Context (thread_own : thread_id → PROP).
+
+  Definition gen_log_rel e_t e_s : PROP :=
+    □ ∀ π (map : gmap string (val Λ * val Λ)),
+      subst_map_rel (free_vars e_t ∪ free_vars e_s) map -∗
+      thread_own π -∗
+      subst_map (fst <$> map) e_t ⪯{π} subst_map (snd <$> map) e_s
+        {{ λ v_t v_s, thread_own π ∗ val_rel v_t v_s }}.
+
+  Global Instance gen_log_rel_persistent e_t e_s : Persistent (gen_log_rel e_t e_s).
+  Proof. rewrite /gen_log_rel; apply _. Qed.
+
+  Lemma gen_log_rel_closed_1 e_t e_s π :
+    free_vars e_t ∪ free_vars e_s = ∅ →
+    gen_log_rel e_t e_s ⊢
+      thread_own π -∗ e_t ⪯{π} e_s {{ λ v_t v_s, thread_own π ∗ val_rel v_t v_s }}.
+  Proof.
+    iIntros (Hclosed) "#Hrel". iSpecialize ("Hrel" $! π ∅).
+    rewrite ->!fmap_empty, ->!subst_map_empty.
+    rewrite Hclosed. iApply "Hrel". by iApply subst_map_rel_empty.
+  Qed.
+
+  Lemma gen_log_rel_closed e_t e_s :
+    free_vars e_t ∪ free_vars e_s = ∅ →
+    gen_log_rel e_t e_s ⊣⊢
+      (□ ∀ π, thread_own π -∗
+        e_t ⪯{π} e_s {{ λ v_t v_s, thread_own π ∗ val_rel v_t v_s }}).
+  Proof.
+    intros Hclosed. iSplit.
+    { iIntros "#Hrel !#" (π). iApply gen_log_rel_closed_1; done. }
+    iIntros "#Hsim" (π xs) "!# Hxs".
+    rewrite !subst_map_closed //; set_solver.
+  Qed.
+
+  Lemma gen_log_rel_singleton e_t e_s v_t v_s arg π :
+    free_vars e_t ∪ free_vars e_s ⊆ {[ arg ]} →
+    gen_log_rel e_t e_s -∗
+    val_rel v_t v_s -∗
+    thread_own π -∗
+    subst_map {[arg := v_t]} e_t ⪯{π} subst_map {[arg := v_s]} e_s
+      {{ λ v_t v_s, thread_own π ∗ val_rel v_t v_s }}.
+  Proof.
+    iIntros (?) "Hlog Hval Hπ".
+    iDestruct ("Hlog" $! _ {[arg := (v_t, v_s)]} with "[Hval] Hπ") as "Hsim".
+    { by iApply subst_map_rel_singleton. }
+    rewrite !map_fmap_singleton. done.
+  Qed.
+
+  (** Substitute away a single free variable in an [gen_log_rel]. *)
+  Lemma gen_log_rel_subst x e_t e_s dummy {HPers : ∀ vt vs, Persistent (val_rel vt vs)} :
+    (* In case [x] is not free, we need a reflexive "default value" *)
+    □ val_rel dummy dummy -∗
+    (□ ∀ (v_t v_s : val Λ), val_rel v_t v_s -∗
+      gen_log_rel (subst_map {[x:=v_t]} e_t) (subst_map {[x:=v_s]} e_s)) -∗
+    gen_log_rel e_t e_s.
+  Proof.
+    iIntros "#Hdummy #Hsim %π %xs !# #Hxs Hπ".
+    destruct (decide (x ∈ free_vars e_t ∪ free_vars e_s)) as [Hin|Hnotin]; last first.
+    { iSpecialize ("Hsim" $! dummy dummy).
+      rewrite ->(subst_map_free_vars _ ∅ e_t); last first.
+      { intros x' ?. assert (x ≠ x') by set_solver.
+        rewrite lookup_singleton_ne //. }
+      rewrite ->(subst_map_free_vars _ ∅ e_s); last first.
+      { intros x' ?. assert (x ≠ x') by set_solver.
+        rewrite lookup_singleton_ne //. }
+      rewrite !subst_map_empty.
+      iApply "Hsim"; eauto. }
+    iDestruct (subst_map_rel_lookup x with "Hxs") as (v_t v_s Hv) "Hrel"; first done.
+    iSpecialize ("Hsim" $! v_t v_s with "Hrel").
+    iSpecialize ("Hsim" $! π xs with "[Hxs]").
+    { iApply (subst_map_rel_weaken with "Hxs").
+      rewrite !free_vars_subst_map. set_solver. }
+    rewrite !subst_map_subst_map.
+    replace ({[x := v_t]} ∪ (fst <$> xs)) with (fst <$> xs); last first.
+    { rewrite -insert_union_singleton_l insert_id //.
+      rewrite lookup_fmap Hv //. }
+    replace ({[x := v_s]} ∪ (snd <$> xs)) with (snd <$> xs); last first.
+    { rewrite -insert_union_singleton_l insert_id //.
+      rewrite lookup_fmap Hv //. }
+    iApply "Hsim"; eauto.
+  Qed.
+
+End fix_lang.
+
+Arguments prog_rel : simpl never.
+Arguments gen_log_rel : simpl never.
+Typeclasses Opaque prog_rel gen_log_rel.
